new/golang/theory/interface.v
@@ -2,6 +2,8 @@ From Perennial.goose_lang Require Import notation.
 From New.golang.theory Require Import struct typing proofmode globals.
 From New.golang.defn Require Import interface globals.
 
+Set Default Proof Using "Type".
+
 Section wps.
 Context `{sem: ffi_semantics} `{!ffi_interp ffi} `{!heapGS Σ}.
 
@@ -48,6 +50,69 @@ Proof.
   destruct i as [|].
   - wp_pures. wp_pures. rewrite bool_decide_false //. by iApply "Hwp".
   - wp_pures. rewrite bool_decide_true //. by iApply "Hwp".
+Qed.
+
+Lemma wp_interface_type_assert (i : interface.t) {V} `{!IntoVal V} pkg_name type_name (x: V) :
+  {{{ ⌜i = interface.mk pkg_name type_name #x⌝ }}}
+    interface.type_assert #i #pkg_name #type_name
+  {{{ RET #x; True }}}.
+Proof.
+  iIntros (Φ) "-> HΦ".
+  wp_call.
+  rewrite {1}[in #(interface.mk _ _ _)]to_val_unseal /=.
+  wp_pures.
+  rewrite bool_decide_eq_true_2 //.
+  wp_pures.
+  rewrite bool_decide_eq_true_2 //.
+  wp_pures.
+  by iApply "HΦ".
+Qed.
+
+Lemma wp_interface_checked_type_assert (i : interface.t) {V} `{!IntoVal V} t `{!IntoValTyped V t}
+  pkg_name type_name :
+  {{{ ⌜match i with
+      | interface.mk pkg_name' type_name' v0 =>
+          (* a technical side condition is required to show that if i has the
+          correct type identity (which is a string), then the value it holds has
+          the expected type V *)
+          (pkg_name', type_name') = (pkg_name, type_name) →
+          ∃ (v: V), v0 = #v
+      |  interface.nil => True
+      end ⌝ }}}
+    interface.checked_type_assert #t #i #pkg_name #type_name
+  {{{ (y: V) (ok: bool), RET (#y, #ok);
+      ⌜if ok then i = interface.mk pkg_name type_name #y
+      else match i with
+      | interface.mk pkg_name' type_name' _ => (pkg_name', type_name') ≠ (pkg_name, type_name)
+      | interface.nil => True
+      end ∧ y = default_val V⌝
+  }}}.
+Proof.
+  iIntros (Φ) "%Htype HΦ".
+  wp_call.
+  destruct i as [pkg_name' type_name' y'|].
+  - rewrite {1}[in #(interface.mk _ _ _)]to_val_unseal /=.
+    wp_pures.
+    destruct (bool_decide_reflect (pkg_name' = pkg_name)); subst; wp_pures.
+    {
+      destruct (bool_decide_reflect (type_name' = type_name)); subst; wp_pures.
+      { destruct Htype as [v ->]; [ done | ].
+        iApply "HΦ".
+        done. }
+      rewrite -default_val_eq_zero_val.
+      iApply "HΦ".
+      iPureIntro.
+      split; congruence.
+    }
+    rewrite -default_val_eq_zero_val.
+    iApply "HΦ".
+    iPureIntro.
+    split; congruence.
+  - rewrite {1}[in #(interface.nil)]to_val_unseal /=.
+    wp_pures.
+    rewrite -default_val_eq_zero_val.
+    iApply "HΦ".
+    done.
 Qed.
 
 End wps.
